Simplify meta usage.

theories/concurrent/counter.v
@@ -53,73 +53,84 @@ Section counter_G.
     λ: "t",
       !"t".
 
-  Notation counter_meta_ub :=
-    (nroot .@ "ub").
-  Notation counter_meta_lb :=
-    (nroot .@ "lb").
-  Notation counter_meta_token :=
-    (nroot .@ "token").
-  Notation counter_meta_model :=
-    (nroot .@ "model").
+  Record counter_name := {
+    counter_name_ub : gname ;
+    counter_name_lb : gname ;
+    counter_name_token : gname ;
+    counter_name_model : gname ;
+  }.
+  #[local] Instance counter_name_eq_dec :
+    EqDecision counter_name.
+  Proof.
+    solve_decision.
+  Qed.
+  #[local] Instance counter_name_countable :
+    Countable counter_name.
+  Proof.
+    pose encode γ := (
+      γ.(counter_name_ub),
+      γ.(counter_name_lb),
+      γ.(counter_name_token),
+      γ.(counter_name_model)
+    ).
+    pose decode := λ '(γ_ub, γ_lb, γ_token, γ_model),
+      Build_counter_name γ_ub γ_lb γ_token γ_model.
+    refine (inj_countable' encode decode _). intros []. done.
+  Qed.
+  Implicit Types γ : counter_name.
 
-  #[local] Definition counter_ub_auth γ_ub ub :=
-    auth_natinf_max_auth γ_ub DfracDiscarded (
+  #[local] Definition counter_ub_auth γ ub :=
+    auth_natinf_max_auth γ.(counter_name_ub) DfracDiscarded (
       if ub is Some ub then natinf_nat ub else natinf_inf
     ).
-  #[local] Definition counter_ub_frag γ_ub n :=
-    auth_natinf_max_frag γ_ub (natinf_nat n).
+  #[local] Definition counter_ub_frag γ n :=
+    auth_natinf_max_frag γ.(counter_name_ub) (natinf_nat n).
 
-  #[local] Definition counter_lb_auth γ_lb dq n :=
-    auth_nat_max_auth γ_lb dq n.
-  #[local] Definition counter_lb_frag γ_lb lb :=
-    auth_nat_max_frag γ_lb lb.
+  #[local] Definition counter_lb_auth γ dq n :=
+    auth_nat_max_auth γ.(counter_name_lb) dq n.
+  #[local] Definition counter_lb_frag γ lb :=
+    auth_nat_max_frag γ.(counter_name_lb) lb.
   Definition counter_lb t lb : iProp Σ :=
-    ∃ l γ_ub γ_lb,
+    ∃ l γ,
     ⌜t = #l⌝ ∗
-    meta l counter_meta_ub γ_ub ∗
-    meta l counter_meta_lb γ_lb ∗
-    counter_ub_frag γ_ub lb ∗
-    counter_lb_frag γ_lb lb.
+    meta l nroot γ ∗
+    counter_ub_frag γ lb ∗
+    counter_lb_frag γ lb.
 
-  #[local] Definition counter_token_auth γ_token dq n :=
-    own γ_token (●{dq} GSet (set_seq 0 n)).
-  #[local] Definition counter_token_frag γ_token n :=
-    own γ_token (◯ GSet {[n]}).
+  #[local] Definition counter_token_auth γ dq n :=
+    own γ.(counter_name_token) (●{dq} GSet (set_seq 0 n)).
+  #[local] Definition counter_token_frag γ n :=
+    own γ.(counter_name_token) (◯ GSet {[n]}).
   Definition counter_token t n : iProp Σ :=
-    ∃ l γ_ub γ_token,
+    ∃ l γ,
     ⌜t = #l⌝ ∗
-    meta l counter_meta_ub γ_ub ∗
-    meta l counter_meta_token γ_token ∗
-    counter_ub_frag γ_ub n ∗
-    counter_token_frag γ_token n.
+    meta l nroot γ ∗
+    counter_ub_frag γ n ∗
+    counter_token_frag γ n.
 
-  #[local] Definition counter_model₁ γ_model n :=
-    auth_excl_frag γ_model n.
-  #[local] Definition counter_model₂ γ_model dq n :=
-    auth_excl_auth γ_model dq n.
+  #[local] Definition counter_model₁ γ n :=
+    auth_excl_frag γ.(counter_name_model) n.
+  #[local] Definition counter_model₂ γ dq n :=
+    auth_excl_auth γ.(counter_name_model) dq n.
   Definition counter_model t dq n : iProp Σ :=
-    ∃ l γ_ub γ_lb γ_token γ_model,
+    ∃ l γ,
     ⌜t = #l⌝ ∗
-    meta l counter_meta_ub γ_ub ∗
-    meta l counter_meta_lb γ_lb ∗
-    meta l counter_meta_token γ_token ∗
-    meta l counter_meta_model γ_model ∗
-    counter_ub_frag γ_ub n ∗
-    counter_lb_auth γ_lb dq n ∗
-    counter_token_auth γ_token dq n ∗
-    counter_model₂ γ_model dq n.
+    meta l nroot γ ∗
+    counter_ub_frag γ n ∗
+    counter_lb_auth γ dq n ∗
+    counter_token_auth γ dq n ∗
+    counter_model₂ γ dq n.
 
-  #[local] Definition counter_inv_inner l γ_model : iProp Σ :=
+  #[local] Definition counter_inv_inner l γ : iProp Σ :=
     ∃ n,
     l ↦ #n ∗
-    counter_model₁ γ_model n.
+    counter_model₁ γ n.
   Definition counter_inv t ι ub : iProp Σ :=
-    ∃ l γ_ub γ_model,
+    ∃ l γ,
     ⌜t = #l⌝ ∗
-    meta l counter_meta_ub γ_ub ∗
-    meta l counter_meta_model γ_model ∗
-    counter_ub_auth γ_ub ub ∗
-    inv ι (counter_inv_inner l γ_model).
+    meta l nroot γ ∗
+    counter_ub_auth γ ub ∗
+    inv ι (counter_inv_inner l γ).
 
   #[global] Instance counter_lb_persistent t lb :
     Persistent (counter_lb t lb).
@@ -151,13 +162,10 @@ Section counter_G.
     Fractional (λ q, counter_model t (DfracOwn q) n).
   Proof.
     intros q1 q2. iSplit.
-    - iIntros "(%l & %γ_ub & %γ_lb & %γ_token & %γ_model & -> & #Hmeta_ub & #Hmeta_lb & #Hmeta_token & #Hmeta_model & #Hub_frag & (Hlb_auth1 & Hlb_auth2) & (Htoken_auth1 & Htoken_auth2) & (Hmodel₂1 & Hmodel₂2))".
+    - iIntros "(%l & %γ & -> & #Hmeta & #Hub_frag & (Hlb_auth1 & Hlb_auth2) & (Htoken_auth1 & Htoken_auth2) & (Hmodel₂1 & Hmodel₂2))".
       iSplitL "Hlb_auth1 Htoken_auth1 Hmodel₂1"; repeat iExists _; iFrame "#∗"; done.
-    - iIntros "((%l & %γ_ub & %γ_lb & %γ_token & %γ_model & -> & #Hmeta_ub & #Hmeta_lb & #Hmeta_token & #Hmeta_model & #Hub_frag & Hlb_auth1 & Htoken_auth1 & Hmodel₂1) & (%_l & %_γ_ub & %_γ_lb & %_γ_token & %_γ_model & %Heq & #_Hmeta_ub & #_Hmeta_lb & #_Hmeta_token & #_Hmeta_model & _ & Hlb_auth2 & Htoken_auth2 & Hmodel₂2))". injection Heq as <-.
-      iDestruct (meta_agree with "Hmeta_ub _Hmeta_ub") as %->. iClear "_Hmeta_ub".
-      iDestruct (meta_agree with "Hmeta_lb _Hmeta_lb") as %->. iClear "_Hmeta_lb".
-      iDestruct (meta_agree with "Hmeta_token _Hmeta_token") as %->. iClear "_Hmeta_token".
-      iDestruct (meta_agree with "Hmeta_model _Hmeta_model") as %->. iClear "_Hmeta_model".
+    - iIntros "((%l & %γ & -> & #Hmeta & #Hub_frag & Hlb_auth1 & Htoken_auth1 & Hmodel₂1) & (%_l & %_γ & %Heq & #_Hmeta & _ & Hlb_auth2 & Htoken_auth2 & Hmodel₂2))". injection Heq as <-.
+      iDestruct (meta_agree with "Hmeta _Hmeta") as %->. iClear "_Hmeta".
       iCombine "Hlb_auth1 Hlb_auth2" as "Hlb_auth".
       iCombine "Htoken_auth1 Htoken_auth2" as "Htoken_auth".
       iCombine "Hmodel₂1 Hmodel₂2" as "Hmodel₂".
@@ -174,8 +182,8 @@ Section counter_G.
     counter_lb t lb -∗
     ⌜lb ≤ ub⌝.
   Proof.
-    iIntros "(%l & %γ_ub & %γ_model & -> & #Hmeta_ub & #Hmeta_model & #Hub_auth & #Hinv) (%_l & %_γ_ub & %_γ_lb & %Heq & #_Hmeta_ub & #_Hmeta_lb & #Hub_frag & #Hlb_frag)". injection Heq as <-.
-    iDestruct (meta_agree with "Hmeta_ub _Hmeta_ub") as %<-. iClear "_Hmeta_ub".
+    iIntros "(%l & %γ & -> & #Hmeta & #Hub_auth & #Hinv) (%_l & %_γ & %Heq & #_Hmeta & #Hub_frag & #Hlb_frag)". injection Heq as <-.
+    iDestruct (meta_agree with "Hmeta _Hmeta") as %<-. iClear "_Hmeta".
     iDestruct (auth_natinf_max_valid with "Hub_auth Hub_frag") as %?%(inj natinf_nat). done.
   Qed.
   Lemma counter_lb_le t lb1 lb2 :
@@ -183,7 +191,7 @@ Section counter_G.
     counter_lb t lb1 -∗
     counter_lb t lb2.
   Proof.
-    iIntros "% (%l & %γ_ub & %γ_lb & -> & #Hmeta_ub & #Hmeta_lb & #Hub_frag & Hlb_frag)".
+    iIntros "% (%l & %γ & -> & #Hmeta & #Hub_frag & Hlb_frag)".
     iDestruct (auth_natinf_max_frag_le with "Hub_frag") as "#Hub_frag'".
     { apply natinf_le_proper. done. }
     iDestruct (auth_nat_max_frag_le with "Hlb_frag") as "Hlb_frag"; first done.
@@ -193,7 +201,7 @@ Section counter_G.
     counter_model t dq n -∗
     counter_lb t n.
   Proof.
-    iIntros "(%l & %γ_ub & %γ_lb & %γ_token & %γ_model & -> & #Hmeta_ub & #Hmeta_lb & #Hmeta_token & #Hmeta_model & #Hub_frag & Hlb_auth & Htoken_auth & Hmodel₂)".
+    iIntros "(%l & %γ & -> & #Hmeta & #Hub_frag & Hlb_auth & Htoken_auth & Hmodel₂)".
     iDestruct (auth_nat_max_frag_get with "Hlb_auth") as "#Hlb_frag".
     repeat iExists _. naive_solver.
   Qed.
@@ -203,8 +211,8 @@ Section counter_G.
     counter_token t n -∗
     ⌜n ≤ ub⌝.
   Proof.
-    iIntros "(%l & %γ_ub & %γ_model & -> & #Hmeta_ub & #Hmeta_model & #Hub_auth & #Hinv) (%_l & %_γ_ub & %_γ_lb & %Heq & #_Hmeta_ub & #_Hmeta_token & #Hub_frag & Htoken_frag)". injection Heq as <-.
-    iDestruct (meta_agree with "Hmeta_ub _Hmeta_ub") as %<-. iClear "_Hmeta_ub".
+    iIntros "(%l & %γ & -> & #Hmeta & #Hub_auth & #Hinv) (%_l & %_γ & %Heq & #_Hmeta & #Hub_frag & Htoken_frag)". injection Heq as <-.
+    iDestruct (meta_agree with "Hmeta _Hmeta") as %<-. iClear "_Hmeta".
     iDestruct (auth_natinf_max_valid with "Hub_auth Hub_frag") as %?%(inj natinf_nat). done.
   Qed.
   Lemma counter_token_exclusive t n :
@@ -212,8 +220,8 @@ Section counter_G.
     counter_token t n -∗
     False.
   Proof.
-    iIntros "(%l & %γ_ub & %γ_token & -> & #Hmeta_ub & #Hmeta_token & #Hub_frag & Htoken_frag1) (%_l & %_γ_ub & %_γ_token & %Heq & #_Hmeta_ub & #_Hmeta_token & _ & Htoken_frag2)". injection Heq as <-.
-    iDestruct (meta_agree with "Hmeta_token _Hmeta_token") as %->. iClear "_Hmeta_token".
+    iIntros "(%l & %γ & -> & #Hmeta & #Hub_frag & Htoken_frag1) (%_l & %_γ & %Heq & #_Hmeta & _ & Htoken_frag2)". injection Heq as <-.
+    iDestruct (meta_agree with "Hmeta _Hmeta") as %->. iClear "_Hmeta".
     iDestruct (own_valid_2 with "Htoken_frag1 Htoken_frag2") as %?%auth_frag_op_valid%gset_disj_valid_op. set_solver.
   Qed.
 
@@ -221,7 +229,7 @@ Section counter_G.
     counter_model t dq n -∗
     ⌜✓ dq⌝.
   Proof.
-    iIntros "(%l & %γ_ub & %γ_lb & %γ_token & %γ_model & -> & #Hmeta_ub & #Hmeta_lb & #Hmeta_token & #Hmeta_model & #Hub_frag & Hlb_auth & Htoken_auth & Hmodel₂)".
+    iIntros "(%l & %γ & -> & #Hmeta & #Hub_frag & Hlb_auth & Htoken_auth & Hmodel₂)".
     iApply (auth_excl_auth_valid with "Hmodel₂").
   Qed.
   Lemma counter_inv_model_valid t ι ub dq n :
@@ -229,9 +237,9 @@ Section counter_G.
     counter_model t dq n -∗
     ⌜if ub is Some ub then n ≤ ub else True⌝.
   Proof.
-    iIntros "(%l & %γ_ub & %γ_model & -> & #Hmeta_ub & #Hmeta_model & #Hub_auth & #Hinv) (%_l & %_γ_ub & %γ_lb & %γ_token & %_γ_model & %Heq & #_Hmeta_ub & #Hmeta_lb & #_Hmeta_token & #_Hmeta_model & #Hub_frag & Hlb_auth & Htoken_auth & Hmodel₂)". injection Heq as <-.
+    iIntros "(%l & %γ & -> & #Hmeta & #Hub_auth & #Hinv) (%_l & %_γ & %Heq & #_Hmeta & #Hub_frag & Hlb_auth & Htoken_auth & Hmodel₂)". injection Heq as <-.
     destruct ub as [ub |]; last done.
-    iDestruct (meta_agree with "Hmeta_ub _Hmeta_ub") as %<-. iClear "_Hmeta_ub".
+    iDestruct (meta_agree with "Hmeta _Hmeta") as %<-. iClear "_Hmeta".
     iDestruct (auth_natinf_max_valid with "Hub_auth Hub_frag") as %?%(inj natinf_nat). done.
   Qed.
   Lemma counter_model_lb_valid t dq n lb :
@@ -239,8 +247,8 @@ Section counter_G.
     counter_lb t lb -∗
     ⌜lb ≤ n⌝.
   Proof.
-    iIntros "(%l & %γ_ub & %γ_lb & %γ_token & %γ_model & -> & #Hmeta_ub & #Hmeta_lb & #Hmeta_token & #Hmeta_model & #Hub_frag & Hlb_auth & Htoken_auth & Hmodel₂) (%_l & %_γ_ub & %_γ_lb & %Heq & #_Hmeta_ub & #_Hmeta_lb & _ & #Hlb_frag)". injection Heq as <-.
-    iDestruct (meta_agree with "Hmeta_lb _Hmeta_lb") as %->. iClear "_Hmeta_lb".
+    iIntros "(%l & %γ & -> & #Hmeta & #Hub_frag & Hlb_auth & Htoken_auth & Hmodel₂) (%_l & %_γ & %Heq & #_Hmeta & _ & #Hlb_frag)". injection Heq as <-.
+    iDestruct (meta_agree with "Hmeta _Hmeta") as %->. iClear "_Hmeta".
     iApply (auth_nat_max_valid with "Hlb_auth Hlb_frag").
   Qed.
   Lemma counter_model_token_valid t dq n m :
@@ -248,8 +256,8 @@ Section counter_G.
     counter_token t m -∗
     ⌜m < n⌝.
   Proof.
-    iIntros "(%l & %γ_ub & %γ_lb & %γ_token & %γ_model & -> & #Hmeta_ub & #Hmeta_lb & #Hmeta_token & #Hmeta_model & #Hub_frag & Hlb_auth & Htoken_auth & Hmodel₂) (%_l & %_γ_ub & %_γ_token & %Heq & #_Hmeta_ub & #_Hmeta_token & _ & Htoken_frag)". injection Heq as <-.
-    iDestruct (meta_agree with "Hmeta_token _Hmeta_token") as %->. iClear "_Hmeta_token".
+    iIntros "(%l & %γ & -> & #Hmeta & #Hub_frag & Hlb_auth & Htoken_auth & Hmodel₂) (%_l & %_γ & %Heq & #_Hmeta & _ & Htoken_frag)". injection Heq as <-.
+    iDestruct (meta_agree with "Hmeta _Hmeta") as %->. iClear "_Hmeta".
     iDestruct (own_valid_2 with "Htoken_auth Htoken_frag") as %(_ & Hincluded & _)%auth_both_dfrac_valid_discrete.
     rewrite gset_disj_included -elem_of_subseteq_singleton elem_of_set_seq in Hincluded.
     naive_solver.
@@ -260,10 +268,8 @@ Section counter_G.
       counter_model t (dq1 ⋅ dq2) n1 ∗
       ⌜n1 = n2⌝.
   Proof.
-    iIntros "(%l & %γ_ub & %γ_lb & %γ_token & %γ_model & -> & #Hmeta_ub & #Hmeta_lb & #Hmeta_token & #Hmeta_model & #Hub_frag1 & Hlb_auth1 & Htoken_auth1 & Hmodel₂1) (%_l & %_γ_ub & %_γ_lb & %_γ_token & %_γ_model & %Heq & #_Hmeta_ub & #_Hmeta_lb & #_Hmeta_token & #_Hmeta_model & #Hub_frag2 & Hlb_auth2 & Htoken_auth2 & Hmodel₂2)". injection Heq as <-.
-    iDestruct (meta_agree with "Hmeta_lb _Hmeta_lb") as %->. iClear "_Hmeta_lb".
-    iDestruct (meta_agree with "Hmeta_token _Hmeta_token") as %->. iClear "_Hmeta_token".
-    iDestruct (meta_agree with "Hmeta_model _Hmeta_model") as %->. iClear "_Hmeta_model".
+    iIntros "(%l & %γ & -> & #Hmeta & #Hub_frag1 & Hlb_auth1 & Htoken_auth1 & Hmodel₂1) (%_l & %_γ & %Heq & #_Hmeta & #Hub_frag2 & Hlb_auth2 & Htoken_auth2 & Hmodel₂2)". injection Heq as <-.
+    iDestruct (meta_agree with "Hmeta _Hmeta") as %->. iClear "_Hmeta".
     iDestruct (auth_nat_max_auth_combine with "Hlb_auth1 Hlb_auth2") as "(Hlb_auth & <-)".
     iCombine "Htoken_auth1 Htoken_auth2" as "Htoken_auth".
     iDestruct (auth_excl_auth_combine_L with "Hmodel₂1 Hmodel₂2") as "(Hmodel₂ & _)".
@@ -315,7 +321,7 @@ Section counter_G.
     counter_model t dq n ==∗
     counter_model t DfracDiscarded n.
   Proof.
-    iIntros "(%l & %γ_ub & %γ_lb & %γ_token & %γ_model & -> & #Hmeta_ub & #Hmeta_lb & #Hmeta_token & #Hmeta_model & #Hub_frag & Hlb_auth & Htoken_auth & Hmodel₂)".
+    iIntros "(%l & %γ & -> & #Hmeta & #Hub_frag & Hlb_auth & Htoken_auth & Hmodel₂)".
     iMod (auth_nat_max_auth_persist with "Hlb_auth") as "Hlb_auth".
     iMod (own_update with "Htoken_auth") as "Htoken_auth"; first eapply auth_update_auth_persist.
     iMod (auth_excl_auth_persist with "Hmodel₂") as "Hmodel₂".
@@ -331,18 +337,17 @@ Section counter_G.
     wp_rec. iApply wp_fupd. wp_apply (wp_alloc with "[//]"). iIntros "%l (Hl & Hmeta)".
     iMod (auth_natinf_max_alloc (if ub is Some ub then natinf_nat ub else natinf_inf)) as "(%γ_ub & Hub_auth)".
     iMod (auth_natinf_max_auth_persist with "Hub_auth") as "Hub_auth".
-    iMod auth_natinf_max_frag_0 as "#Hub_frag".
+    iMod (auth_natinf_max_frag_0 γ_ub) as "#Hub_frag".
     iMod (auth_nat_max_alloc 0) as "(%γ_lb & Hlb_auth)".
     iMod (own_alloc (● GSet ∅)) as "(%γ_token & Htoken_auth)"; first by apply auth_auth_valid.
     iMod (auth_excl_alloc' (auth_excl_G := counter_G_model_G) 0) as "(%γ_model & Hmodel₂ & Hmodel₁)".
-    iDestruct (meta_token_difference _ (↑counter_meta_ub) with "Hmeta") as "(Hmeta_ub & Hmeta)"; first solve_ndisj.
-    iDestruct (meta_token_difference _ (↑counter_meta_lb) with "Hmeta") as "(Hmeta_lb & Hmeta)"; first solve_ndisj.
-    iDestruct (meta_token_difference _ (↑counter_meta_token) with "Hmeta") as "(Hmeta_token & Hmeta)"; first solve_ndisj.
-    iDestruct (meta_token_difference _ (↑counter_meta_model) with "Hmeta") as "(Hmeta_model & Hmeta)"; first solve_ndisj.
-    iMod (meta_set _ _ γ_ub with "Hmeta_ub") as "#Hmeta_ub"; first done.
-    iMod (meta_set _ _ γ_lb with "Hmeta_lb") as "#Hmeta_lb"; first done.
-    iMod (meta_set _ _ γ_token with "Hmeta_token") as "#Hmeta_token"; first done.
-    iMod (meta_set _ _ γ_model with "Hmeta_model") as "#Hmeta_model"; first done.
+    set γ := {|
+      counter_name_ub := γ_ub ;
+      counter_name_lb := γ_lb ;
+      counter_name_token := γ_token ;
+      counter_name_model := γ_model ;
+    |}.
+    iMod (meta_set _ _ γ with "Hmeta") as "#Hmeta"; first done.
     iApply "HΦ". iSplitL "Hub_auth Hl Hmodel₁".
     - repeat iExists _. iFrame "#∗". iSplitR; first done.
       iApply inv_alloc. iExists 0. iFrame.
@@ -360,13 +365,12 @@ Section counter_G.
       RET #n; True
     >>>.
   Proof.
-    iIntros "!> %Φ (%l & %γ_ub & %γ_model & -> & #Hmeta_ub & #Hmeta_model & #Hub_auth & #Hinv) HΦ".
+    iIntros "!> %Φ (%l & %γ & -> & #Hmeta & #Hub_auth & #Hinv) HΦ".
     wp_rec.
     iInv "Hinv" as "(%n & Hl & Hmodel₁)".
     wp_faa.
-    iMod "HΦ" as "(%_n & ((%_l & %_γ_ub & %γ_lb & %γ_token & %_γ_model & %Heq & #_Hmeta_ub & #Hmeta_lb & #Hmeta_token & #_Hmeta_model & #Hub_frag & Hlb_auth & Htoken_auth & Hmodel₂) & #Hle) & _ & HΦ)". injection Heq as <-.
-    iDestruct (meta_agree with "Hmeta_ub _Hmeta_ub") as %<-. iClear "_Hmeta_ub".
-    iDestruct (meta_agree with "Hmeta_model _Hmeta_model") as %<-. iClear "_Hmeta_model".
+    iMod "HΦ" as "(%_n & ((%_l & %_γ & %Heq & #_Hmeta & #Hub_frag & Hlb_auth & Htoken_auth & Hmodel₂) & #Hle) & _ & HΦ)". injection Heq as <-.
+    iDestruct (meta_agree with "Hmeta _Hmeta") as %<-. iClear "_Hmeta".
     iDestruct (auth_excl_agree_L with "Hmodel₂ Hmodel₁") as %->.
     iMod (auth_nat_max_update (S n) with "Hlb_auth") as "Hlb_auth"; first lia.
     iMod (own_update _ _ (● GSet (set_seq 0 (S n)) ⋅ ◯ GSet {[n]}) with "Htoken_auth") as "(Htoken_auth & Htoken_frag)".
@@ -402,13 +406,12 @@ Section counter_G.
       RET #n; if ub is Some ub then ⌜n ≤ ub⌝ else True
     >>>.
   Proof.
-    iIntros "!> %Φ (%l & %γ_ub & %γ_model & -> & #Hmeta_ub & #Hmeta_model & #Hub_auth & #Hinv) HΦ".
+    iIntros "!> %Φ (%l & %γ & -> & #Hmeta & #Hub_auth & #Hinv) HΦ".
     wp_rec.
     iInv "Hinv" as "(%n & Hl & Hmodel₁)".
     wp_load.
-    iMod "HΦ" as "(%dq & %_n & (%_l & %_γ_ub & %γ_lb & %γ_token & %_γ_model & %Heq & #_Hmeta_ub & #Hmeta_lb & #Hmeta_token & #_Hmeta_model & #Hub_frag & Hlb_auth & Htoken_auth & Hmodel₂) & _ & HΦ)". injection Heq as <-.
-    iDestruct (meta_agree with "Hmeta_ub _Hmeta_ub") as %<-. iClear "_Hmeta_ub".
-    iDestruct (meta_agree with "Hmeta_model _Hmeta_model") as %<-. iClear "_Hmeta_model".
+    iMod "HΦ" as "(%dq & %_n & (%_l & %_γ & %Heq & #_Hmeta & #Hub_frag & Hlb_auth & Htoken_auth & Hmodel₂) & _ & HΦ)". injection Heq as <-.
+    iDestruct (meta_agree with "Hmeta _Hmeta") as %<-. iClear "_Hmeta".
     iDestruct (auth_excl_agree_L with "Hmodel₂ Hmodel₁") as %->.
     iAssert (counter_model #l dq n) with "[Hlb_auth Htoken_auth Hmodel₂]" as "Hmodel".
     { repeat iExists _. iFrame "#∗". done. }
@@ -423,7 +426,7 @@ Section counter_G.
     counter_inv t ι ub -∗
     ⌜val_is_unboxed t⌝.
   Proof.
-    iIntros "(%l & %γ_ub & %γ_model & -> & #Hmeta_ub & #Hmeta_model & #Hub_auth & #Hinv) //".
+    iIntros "(%l & %γ & -> & #Hmeta & #Hub_auth & #Hinv) //".
   Qed.
 End counter_G.
 
